few more cases

SP1Chips/AddChip.lean
@@ -11,82 +11,88 @@ open LeanRV64D.Functions BitVec
 namespace Add
 
 variable
-  (Main : Vector (Fin BB) 33)
+  (Main : Vector (Fin BB) 34)
   (s : SailState)
   (cstrs : (constraints Main).allHold)
-  (h_is_real : Main[32] = 1)
+  (h_is_real : Main[33] = 1)
 
 noncomputable def spec_add (rs2 rs1 rd : regidx) : SailM Unit := do
   Sail.writeReg Register.nextPC ((← Sail.readReg Register.PC) + 4#64)
   _ ← execute_RTYPE rs2 rs1 rd rop.ADD
   pure ()
 
-def sp1_op_a : BitVec 5 :=
-  by
-    refine BitVec.ofNatLT Main[6] ?_
-    simp
-    show Main[6] < 32
+def sp1_op_a : BitVec 5 := BitVec.ofNat 5 Main[6]
+  -- by
+  --   refine BitVec.ofNatLT Main[6] ?_
+  --   simp
+  --   show Main[6] < 32
 
-    have reader_cstrs := by
-      simp [SP1ConstraintList.allHold, constraints, SP1Constraint.toProp] at cstrs
-      exact cstrs.2.2.1
+  --   have reader_cstrs := by
+  --     simp [SP1ConstraintList.allHold, constraints, SP1Constraint.toProp] at cstrs
+  --     exact cstrs.2.2.1
 
-    clear cstrs
-    simp [RTypeReader.constraints, h_is_real, Opcode.ofNat, Nat.ble, Nat.beq, SP1Constraint.toProp] at reader_cstrs
+  --   clear cstrs
+  --   simp [RTypeReader.constraints, h_is_real, Opcode.ofNat, Nat.ble, Nat.beq, SP1Constraint.toProp] at reader_cstrs
+  --   simp_all only
+  --   exact reader_cstrs.1.2.1
 
-    exact reader_cstrs.1.2.1
+def sp1_op_b : BitVec 5 := BitVec.ofNat 5 Main[14]
+  -- by
+  --   refine BitVec.ofNatLT Main[14] ?_
+  --   simp
+  --   show Main[14] < 32
 
-def sp1_op_b : BitVec 5 :=
-  by
-    refine BitVec.ofNatLT Main[14] ?_
-    simp
-    show Main[14] < 32
+  --   have reader_cstrs := by
+  --     simp [SP1ConstraintList.allHold, constraints, SP1Constraint.toProp] at cstrs
+  --     exact cstrs.2.2.1
 
-    have reader_cstrs := by
-      simp [SP1ConstraintList.allHold, constraints, SP1Constraint.toProp] at cstrs
-      exact cstrs.2.2.1
+  --   clear cstrs
+  --   simp [RTypeReader.constraints, h_is_real, Opcode.ofNat, Nat.ble, Nat.beq, SP1Constraint.toProp] at reader_cstrs
 
-    clear cstrs
-    simp [RTypeReader.constraints, h_is_real, Opcode.ofNat, Nat.ble, Nat.beq, SP1Constraint.toProp] at reader_cstrs
+  --   exact reader_cstrs.1.1.1
 
-    exact reader_cstrs.1.1.1
+def sp1_op_c : BitVec 5 := BitVec.ofNat 5 Main[21]
+  -- by
+  --   refine BitVec.ofNatLT Main[21] ?_
+  --   simp
+  --   show Main[21] < 32
 
-def sp1_op_c : BitVec 5 :=
-  by
-    refine BitVec.ofNatLT Main[21] ?_
-    simp
-    show Main[21] < 32
+  --   have reader_cstrs := by
+  --     simp [SP1ConstraintList.allHold, constraints, SP1Constraint.toProp] at cstrs
+  --     exact cstrs.2.2.1
 
-    have reader_cstrs := by
-      simp [SP1ConstraintList.allHold, constraints, SP1Constraint.toProp] at cstrs
-      exact cstrs.2.2.1
+  --   clear cstrs
+  --   simp [RTypeReader.constraints, h_is_real, Opcode.ofNat, Nat.ble, Nat.beq, SP1Constraint.toProp] at reader_cstrs
 
-    clear cstrs
-    simp [RTypeReader.constraints, h_is_real, Opcode.ofNat, Nat.ble, Nat.beq, SP1Constraint.toProp] at reader_cstrs
-
-    exact reader_cstrs.1.1.2
+  --   exact reader_cstrs.1.1.2
 
 def sp1_add : SailM Unit := do
-  let op_a := sp1_op_a Main cstrs h_is_real
+  let op_a := sp1_op_a Main --cstrs h_is_real
   Sail.writeReg Register.nextPC (Word.toBitVec64 #v[Main[3] + 4, Main[4], Main[5], 0])
-  Sail.write_reg op_a (Word.toBitVec64 #v[Main[28], Main[29], Main[30], Main[31]])
+  Sail.write_reg op_a (Word.toBitVec64 #v[Main[29], Main[30], Main[31], Main[32]])
 
 open Sail
 
 set_option pp.parens true in
 theorem correct_add
+  (Main : Vector (Fin BB) 34)
+  (s : SailState)
+  (cstrs : (constraints Main).allHold)
+  (h_is_real : Main[33] = 1)
   (state_cstrs : (constraints Main).initialState s) :
-  let op_c := sp1_op_c Main cstrs h_is_real
-  let op_b := sp1_op_b Main cstrs h_is_real
-  let op_a := sp1_op_a Main cstrs h_is_real
-  (spec_add (.Regidx op_c) (.Regidx op_b) (.Regidx op_a)).run s = (sp1_add Main cstrs h_is_real).run s
+  let op_c := sp1_op_c Main --cstrs h_is_real
+  let op_b := sp1_op_b Main --cstrs h_is_real
+  let op_a := sp1_op_a Main --cstrs h_is_real
+  (spec_add (.Regidx op_c) (.Regidx op_b) (.Regidx op_a)).run s = (sp1_add Main).run s
   := by
-    simp [SP1ConstraintList.initialState, constraints, SP1Constraint.toStateProp, List.Forall, AddOperation.constraints, CPUState.constraints, RTypeReader.constraints, h_is_real] at state_cstrs
+    simp [SP1ConstraintList.initialState, constraints, SP1Constraint.toStateProp, List.Forall, AddOperation.constraints, CPUState.constraints, RTypeReader.constraints] at state_cstrs
     obtain ⟨read_pc, trusted_instr_state, _, read_op_b, read_op_c⟩ := state_cstrs
     simp [constraints] at cstrs
     obtain ⟨add_op_cstrs, cpu_cstrs, reader_cstrs, rest⟩ := cstrs
     rw [CPUState.allHold_constraints_iff_is_real h_is_real] at cpu_cstrs
     rw [RTypeReader.allHold_constraints_iff_is_real h_is_real] at reader_cstrs
+    simp [Opcode.ofNat, Nat.ble] at reader_cstrs
+    stop
     obtain ⟨ trusted_instr_prop, _, _, _, _, _, _, ⟨ ⟨ _, _, ⟨ _, is_U64_b, is_U64_c ⟩ ⟩, _ ⟩⟩ := reader_cstrs
     simp [Opcode.ofNat, Nat.ble] at trusted_instr_state trusted_instr_prop
 
