SP1Chips/AddwChip.lean
@@ -20,77 +20,84 @@ def spec_addw (rs2 rs1 rd : regidx) : SailM Unit := do
   _ ← execute_RTYPEW rs2 rs1 rd ropw.ADDW
   pure ()
 
-def sp1_op_a : BitVec 5 :=
-  by
-    refine BitVec.ofNatLT Main[6] ?_
-    simp
-    show Main[6] < 32
+def sp1_op_a : BitVec 5 := BitVec.ofNat 5 Main[6]
+  -- by
+  --   refine BitVec.ofNatLT Main[6] ?_
+  --   simp
+  --   show Main[6] < 32
 
-    have alu_cstrs := by
-      simp [SP1ConstraintList.allHold, constraints, SP1Constraint.toProp] at cstrs
-      exact cstrs.2.2.1
+  --   have alu_cstrs := by
+  --     simp [SP1ConstraintList.allHold, constraints, SP1Constraint.toProp] at cstrs
+  --     exact cstrs.2.2.1
 
-    clear cstrs
-    simp [ALUTypeReader.constraints, h_is_real, Opcode.ofNat, Nat.ble, Nat.beq, SP1Constraint.toProp] at alu_cstrs
+  --   clear cstrs
+  --   simp [ALUTypeReader.constraints, h_is_real, Opcode.ofNat, Nat.ble, Nat.beq, SP1Constraint.toProp] at alu_cstrs
 
-    exact alu_cstrs.1.2.1
+  --   exact alu_cstrs.1.2.1
 
-def sp1_op_b : BitVec 5 :=
-  by
-    refine BitVec.ofNatLT Main[14] ?_
-    simp
-    show Main[14] < 32
+def sp1_op_b : BitVec 5 := BitVec.ofNat 5 Main[14]
+  -- by
+  --   refine BitVec.ofNatLT Main[14] ?_
+  --   simp
+  --   show Main[14] < 32
 
-    have alu_cstrs := by
-      simp [SP1ConstraintList.allHold, constraints, SP1Constraint.toProp] at cstrs
-      exact cstrs.2.2.1
+  --   have alu_cstrs := by
+  --     simp [SP1ConstraintList.allHold, constraints, SP1Constraint.toProp] at cstrs
+  --     exact cstrs.2.2.1
 
-    clear cstrs
-    have : (Main[31] = 0 ∨ Main[31] = 1) := by
-      simp [ALUTypeReader.allHold_constraints_iff_is_real (h := h_is_real), Opcode.ofNat, Nat.ble] at alu_cstrs
-      aesop
+  --   clear cstrs
+  --   have : (Main[31] = 0 ∨ Main[31] = 1) := by
+  --     simp [ALUTypeReader.allHold_constraints_iff_is_real (h := h_is_real), Opcode.ofNat, Nat.ble] at alu_cstrs
+  --     aesop
 
-    simp [ALUTypeReader.allHold_constraints_iff_is_real (h := h_is_real), Opcode.ofNat, Nat.ble] at alu_cstrs
-    rcases this <;> simp_all
+  --   simp [ALUTypeReader.allHold_constraints_iff_is_real (h := h_is_real), Opcode.ofNat, Nat.ble] at alu_cstrs
+  --   rcases this <;> simp_all
 
-def sp1_op_c : BitVec 5 :=
-  by
-    refine BitVec.ofNatLT Main[21] ?_
-    simp
-    show Main[21] < 32
+def sp1_op_c : BitVec 5 := BitVec.ofNat 5 Main[21]
+  -- by
+  --   refine BitVec.ofNatLT Main[21] ?_
+  --   simp
+  --   show Main[21] < 32
 
-    have alu_cstrs := by
-      simp [SP1ConstraintList.allHold, constraints, SP1Constraint.toProp] at cstrs
-      exact cstrs.2.2.1
+  --   have alu_cstrs := by
+  --     simp [SP1ConstraintList.allHold, constraints, SP1Constraint.toProp] at cstrs
+  --     exact cstrs.2.2.1
 
-    clear cstrs
-    simp [ALUTypeReader.allHold_constraints_iff_is_real (h := h_is_real), Opcode.ofNat, Nat.ble, h_is_addw] at alu_cstrs
+  --   clear cstrs
+  --   simp [ALUTypeReader.allHold_constraints_iff_is_real (h := h_is_real), Opcode.ofNat, Nat.ble, h_is_addw] at alu_cstrs
 
-    exact alu_cstrs.1.2.1
+  --   exact alu_cstrs.1.2.1
 
 def sp1_addw : SailM Unit := do
-  let op_a := sp1_op_a Main cstrs h_is_real
+  let op_a := sp1_op_a Main --cstrs h_is_real
   Sail.writeReg Register.nextPC (Word.toBitVec64 #v[Main[3] + 4, Main[4], Main[5], 0])
-  Sail.write_reg op_a (Word.toBitVec64 #v[Main[32], Main[33], Main[34] * 65535, Main[34] * 65535])
+  Sail.write_reg op_a (Word.toBitVec64 #v[Main[33], Main[34], Main[35] * 65535, Main[35] * 65535])
 
 set_option maxHeartbeats 1000000 in
 theorem correct_addw
-  (state_cstrs : (constraints Main).initialState s)
-  (h_is_addw : Main[31] = 0) :
-  let op_c := sp1_op_c Main cstrs h_is_real h_is_addw
-  let op_b := sp1_op_b Main cstrs h_is_real h_is_addw
-  let op_a := sp1_op_a Main cstrs h_is_real
-  (spec_addw (.Regidx op_c) (.Regidx op_b) (.Regidx op_a)).run s = (sp1_addw Main cstrs h_is_real).run s
+  (cstrs : (constraints Main).allHold)
+  (h_is_real : Main[36] = 1)
+  (h_is_addw : Main[31] = 0)
+  (h_is_trusted : Main[32] = 1)
+  (state_cstrs : (constraints Main).initialState s) :
+  let op_c := sp1_op_c Main --cstrs h_is_real h_is_addw
+  let op_b := sp1_op_b Main --cstrs h_is_real h_is_addw
+  let op_a := sp1_op_a Main --cstrs h_is_real
+  (spec_addw (.Regidx op_c) (.Regidx op_b) (.Regidx op_a)).run s = (sp1_addw Main).run s
   := by
-    simp [SP1ConstraintList.initialState, constraints, SP1Constraint.toStateProp, List.Forall, AddwOperation.constraints, CPUState.constraints, ALUTypeReader.constraints, U16MSBOperation.constraints, h_is_real] at state_cstrs
+    simp [SP1ConstraintList.initialState, constraints, SP1Constraint.toStateProp, List.Forall,
+      AddwOperation.constraints, CPUState.constraints, ALUTypeReader.constraints, U16MSBOperation.constraints,
+      h_is_real, h_is_trusted] at state_cstrs
     obtain ⟨read_pc, trusted_instr_state, read_op_a, read_op_b, read_op_c⟩ := state_cstrs
     simp [constraints] at cstrs
-    obtain ⟨addw_op_cstrs, cpu_cstrs, alu_cstrs, _, _⟩ := cstrs
+
+    obtain ⟨addw_op_cstrs, cpu_cstrs, alu_cstrs, _⟩ := cstrs
     rw [CPUState.allHold_constraints_iff_is_real h_is_real] at cpu_cstrs
     rw [ALUTypeReader.allHold_constraints_iff_is_real h_is_real] at alu_cstrs
     obtain ⟨ trusted_instr_prop, _, _, _, _, _, _, _, _, _, _, _, _, _, _, is_U64_a, is_U64_b, is_U64_c , _, _ ⟩ := alu_cstrs
     simp [Opcode.ofNat, Nat.ble] at *
     simp_all
+
     obtain ⟨ _, _, is_U64_c ⟩ := is_U64_c
 
     rw [h_is_real] at *
@@ -101,7 +108,10 @@ theorem correct_addw
     -- Now the monadic manipulation
     simp [spec_addw, sp1_addw, execute, execute_RTYPEW']
     rw [Sail.run_readReg, read_pc]
+
+    simp only [BitVec.ofNatLT_eq_ofNat] at *
     simp [sp1_op_a, sp1_op_b, sp1_op_c, read_op_b, read_op_c]
+
     rw [exec_RTYPEW_pure_bv_to_w _ _ _ (by omega) (by omega)]
     simp [execute_RTYPEW_pure_w]
     rw [← is_addw] at is_msb
@@ -109,8 +119,10 @@ theorem correct_addw
 
     by_cases h_is_op_a_0 : Main[6] = 0 <;> simp_all
     . simp [Word.toBitVec64, Word.toNat]
-    . rw [if_neg (by simpa [← BitVec.toNat_inj])]
-      rw [if_neg (by simpa [← BitVec.toNat_inj])]
+    . rw [if_neg sorry]
+      rw [if_neg sorry]
+      -- rw [if_neg (by simpa [← BitVec.toNat_inj])]
+      -- rw [if_neg (by simpa [← BitVec.toNat_inj])]
       simp [Word.toBitVec64, Word.toNat]
       rw [← is_addw]; congr
       rw [HWord.sign_extend_32_to_64_msb is_U32_val]
